Added new tests. Updated agents theory.

eve/Src/Delivery/studio/tools/autoproof/agents.bpl
@@ -1,159 +1,98 @@
 // ----------------------------------------------------------------------
 // Agent theory
 
+const unique ROUTINE: Type;
+axiom (ROUTINE <: ANY);
+
+const unique PROCEDURE: Type;
+axiom (PROCEDURE <: ROUTINE);
+
+const unique FUNCTION: Type;
+axiom (FUNCTION <: ROUTINE);
+
 // Precondition functions for different number of arguments
 
 function routine.precondition_0 (heap: HeapType, agent: ref) returns (bool);
-function routine.precondition_1<arg1Type> (heap: HeapType, agent: ref, arg1: arg1Type) returns (bool);
-function routine.precondition_2<arg1Type, arg2Type> (heap: HeapType, agent: ref, arg1: arg1Type, arg2: arg2Type) returns (bool);
-function routine.precondition_3<arg1Type, arg2Type, arg3Type> (heap: HeapType, agent: ref, arg1: arg1Type, arg2: arg2Type, arg3: arg3Type) returns (bool);
+function routine.precondition_1<T1> (heap: HeapType, agent: ref, arg1: T1) returns (bool);
+function routine.precondition_2<T1, T2> (heap: HeapType, agent: ref, arg1: T1, arg2: T2) returns (bool);
 
 // Postcondition functions for different number of arguments
 
 function routine.postcondition_0 (heap: HeapType, old_heap: HeapType, agent: ref) returns (bool);
-function routine.postcondition_1<arg1Type> (heap: HeapType, old_heap: HeapType, agent: ref, arg1: arg1Type) returns (bool);
-function routine.postcondition_2<arg1Type, arg2Type> (heap: HeapType, old_heap: HeapType, agent: ref, arg1: arg1Type, arg2: arg2Type) returns (bool);
-function routine.postcondition_3<arg1Type, arg2Type, arg3Type> (heap: HeapType, old_heap: HeapType, agent: ref, arg1: arg1Type, arg2: arg2Type, arg3: arg3Type) returns (bool);
+function routine.postcondition_1<T1> (heap: HeapType, old_heap: HeapType, agent: ref, arg1: T1) returns (bool);
+function routine.postcondition_2<T1, T2> (heap: HeapType, old_heap: HeapType, agent: ref, arg1: T1, arg2: T2) returns (bool);
 
 // Postcondition functions for different number of arguments and return values
 
-function function.postcondition_0<resultType> (heap: HeapType, old_heap: HeapType, agent: ref, result: resultType) returns (bool);
-function function.postcondition_1<arg1Type, resultType> (heap: HeapType, old_heap: HeapType, agent: ref, arg1: arg1Type, result: resultType) returns (bool);
-function function.postcondition_2<arg1Type, arg2Type, resultType> (heap: HeapType, old_heap: HeapType, agent: ref, arg1: arg1Type, arg2: arg2Type, result: resultType) returns (bool);
-function function.postcondition_3<arg1Type, arg2Type, arg3Type, resultType> (heap: HeapType, old_heap: HeapType, agent: ref, arg1: arg1Type, arg2: arg2Type, arg3: arg3Type, result: resultType) returns (bool);
+function function.postcondition_0<R> (heap: HeapType, old_heap: HeapType, agent: ref, result: R) returns (bool);
+function function.postcondition_1<T1, R> (heap: HeapType, old_heap: HeapType, agent: ref, arg1: T1, result: R) returns (bool);
+function function.postcondition_2<T1, T2, R> (heap: HeapType, old_heap: HeapType, agent: ref, arg1: T1, arg2: T2, result: R) returns (bool);
 
 // Frame condition function
 
-function agent.modifies_0<alpha> (heap: HeapType, old_heap: HeapType, agent: ref, $o: ref, $f: Field alpha) returns (bool);
-function agent.modifies_1<alpha, arg1Type> (heap: HeapType, old_heap: HeapType, agent: ref, arg1: arg1Type, $o: ref, $f: Field alpha) returns (bool);
-function agent.modifies_2<alpha, arg1Type, arg2Type> (heap: HeapType, old_heap: HeapType, agent: ref, arg1: arg1Type, arg2: arg2Type, $o: ref, $f: Field alpha) returns (bool);
-function agent.modifies_3<alpha, arg1Type, arg2Type, arg3Type> (heap: HeapType, old_heap: HeapType, agent: ref, arg1: arg1Type, arg2: arg2Type, arg3: arg3Type, $o: ref, $f: Field alpha) returns (bool);
-
-// Agents are not changing the reference to themselves...
-axiom (forall<alpha> heap: HeapType, old_heap: HeapType, $a: ref, $o: ref, $f: Field alpha ::
-			{ agent.modifies_0(heap, old_heap, $a, $o, $f) }
-		old_heap[$o, $f] == $a ==> (agent.modifies_0(heap, old_heap, $a, $o, $f) ==> false));
-axiom (forall<alpha, arg1Type> heap: HeapType, old_heap: HeapType, $a: ref, arg1: arg1Type, $o: ref, $f: Field alpha ::
-			{ agent.modifies_1(heap, old_heap, $a, arg1, $o, $f) }
-		old_heap[$o, $f] == $a ==> (agent.modifies_1(heap, old_heap, $a, arg1, $o, $f) ==> false));
-axiom (forall<alpha, arg1Type, arg2Type> heap: HeapType, old_heap: HeapType, $a: ref, arg1: arg1Type, arg2: arg2Type, $o: ref, $f: Field alpha ::
-			{ agent.modifies_2(heap, old_heap, $a, arg1, arg2, $o, $f) }
-		old_heap[$o, $f] == $a ==> (agent.modifies_2(heap, old_heap, $a, arg1, arg2, $o, $f) ==> false));
-axiom (forall<alpha, arg1Type, arg2Type, arg3Type> heap: HeapType, old_heap: HeapType, $a: ref, arg1: arg1Type, arg2: arg2Type, arg3: arg3Type, $o: ref, $f: Field alpha ::
-			{ agent.modifies_3(heap, old_heap, $a, arg1, arg2, arg3, $o, $f) }
-		old_heap[$o, $f] == $a ==> (agent.modifies_3(heap, old_heap, $a, arg1, arg2, arg3, $o, $f) ==> false));
-
-
-// Agent creation
-
-procedure routine.create(
-        Current: ref where Current != Void && !Heap[Current,$allocated]    // The agent object
-    );
-    modifies Heap;
-    // Frame condition
-    ensures frame.modifies_current (Heap, old(Heap), Current);
-    // Object allocated
-    free ensures Heap[Current, $allocated];
+function routine.modify_0 (heap: HeapType, agent: ref) returns (Frame);
+function routine.modify_1<T1> (heap: HeapType, agent: ref, arg1: T1) returns (Frame);
+function routine.modify_2<T1, T2> (heap: HeapType, agent: ref, arg1: T1, arg2: T2) returns (Frame);
 
 // Call functions for different number of arguments
 
-procedure routine.call_0 (
-        Current: ref where Current != Void && Heap[Current,$allocated]     // The agent object
-    );
-    requires routine.precondition_0(Heap, Current); // pre ROUTINE:call tag:precondition
-    modifies Heap;
-    ensures (forall<alpha> $o: ref, $f: Field alpha :: { Heap[$o, $f] } ($o != Void && old(Heap)[$o, $allocated] && !agent.modifies_0(Heap, old(Heap), Current, $o, $f)) ==> (old(Heap)[$o, $f] == Heap[$o, $f])); // frame ROUTINE:call
-    ensures routine.postcondition_0(Heap, old(Heap), Current);
+procedure routine.call_0 (Current: ref);
+  requires attached(Heap, Current, ROUTINE); // info:type property for argument Current
+  requires routine.precondition_0(Heap, Current); // type:pre tag:routine_precondition R1
+  modifies Heap;
+  ensures routine.postcondition_0(Heap, old(Heap), Current);
+  free ensures global(Heap);
+  requires Frame#Subset(routine.modify_0(Heap, Current), writable); // type:pre tag:frame_writable
+  free ensures same_outside(old(Heap), Heap, routine.modify_0(old(Heap), Current));
+  free ensures HeapSucc(old(Heap), Heap);
 
-procedure routine.call_1<arg1Type> (
-        Current: ref where Current != Void && Heap[Current,$allocated],     // The agent object
-        arg1: arg1Type                                                           // First argument
-    );
-    requires routine.precondition_1(Heap, Current, arg1); // pre ROUTINE:call tag:precondition
-    modifies Heap;
-    ensures (forall<alpha> $o: ref, $f: Field alpha :: { Heap[$o, $f] } ($o != Void && old(Heap)[$o, $allocated] && !agent.modifies_1(Heap, old(Heap), Current, arg1, $o, $f)) ==> (old(Heap)[$o, $f] == Heap[$o, $f])); // frame ROUTINE:call
-    ensures routine.postcondition_1(Heap, old(Heap), Current, arg1);
+procedure routine.call_1<T1> (Current: ref, arg1: T1);
+  requires attached(Heap, Current, ROUTINE); // info:type property for argument Current
+  requires routine.precondition_1(Heap, Current, arg1); // type:pre tag:routine_precondition R1
+  modifies Heap;
+  ensures routine.postcondition_1(Heap, old(Heap), Current, arg1);
+  free ensures global(Heap);
+  requires Frame#Subset(routine.modify_1(Heap, Current, arg1), writable); // type:pre tag:frame_writable
+  free ensures same_outside(old(Heap), Heap, routine.modify_1(old(Heap), Current, arg1));
+  free ensures HeapSucc(old(Heap), Heap);
 
-procedure routine.call_2<arg1Type, arg2Type> (
-        Current: ref where Current != Void && Heap[Current,$allocated],     // The agent object
-        arg1: arg1Type,                                                          // First argument
-        arg2: arg2Type// Second argument
-    );
-    requires routine.precondition_2(Heap, Current, arg1, arg2); // pre ROUTINE:call tag:precondition
-    modifies Heap;
-    ensures (forall<alpha> $o: ref, $f: Field alpha :: { Heap[$o, $f] } ($o != Void && old(Heap)[$o, $allocated] && !agent.modifies_2(Heap, old(Heap), Current, arg1, arg2, $o, $f)) ==> (old(Heap)[$o, $f] == Heap[$o, $f])); // frame ROUTINE:call
-    ensures routine.postcondition_2(Heap, old(Heap), Current, arg1, arg2);
+procedure routine.call_2<T1, T2> (Current: ref, arg1: T1, arg2: T2);
+  requires attached(Heap, Current, ROUTINE); // info:type property for argument Current
+  requires routine.precondition_2(Heap, Current, arg1, arg2); // pre ROUTINE:call tag:precondition
+  modifies Heap;
+  ensures routine.postcondition_2(Heap, old(Heap), Current, arg1, arg2);
+  free ensures global(Heap);
+  requires Frame#Subset(routine.modify_2(Heap, Current, arg1, arg2), writable); // type:pre tag:frame_writable
+  free ensures same_outside(old(Heap), Heap, routine.modify_2(old(Heap), Current, arg1, arg2));
+  free ensures HeapSucc(old(Heap), Heap);
 
-procedure routine.call_3<arg1Type, arg2Type, arg3Type> (
-        Current: ref where Current != Void && Heap[Current,$allocated],     // The agent object
-        arg1: arg1Type,                                                          // First argument
-        arg2: arg2Type,                                                          // Second argument
-        arg3: arg3Type                                                           // Third argument
-    );
-    requires routine.precondition_3(Heap, Current, arg1, arg2, arg3); // pre ROUTINE:call tag:precondition
-    modifies Heap;
-    ensures (forall<alpha> $o: ref, $f: Field alpha :: { Heap[$o, $f] } ($o != Void && old(Heap)[$o, $allocated] && !agent.modifies_3(Heap, old(Heap), Current, arg1, arg2, arg3, $o, $f)) ==> (old(Heap)[$o, $f] == Heap[$o, $f])); // frame ROUTINE:call
-    ensures routine.postcondition_3(Heap, old(Heap), Current, arg1, arg2, arg3);
+procedure function.item_0<R> (Current: ref) returns (Result: R);
+  requires attached(Heap, Current, FUNCTION); // info:type property for argument Current
+  requires routine.precondition_0(Heap, Current);
+  modifies Heap;
+  ensures function.postcondition_0(Heap, old(Heap), Current, Result);
+  requires Frame#Subset(routine.modify_0(Heap, Current), writable); // type:pre tag:frame_writable
+  free ensures same_outside(old(Heap), Heap, routine.modify_0(old(Heap), Current));
+  free ensures HeapSucc(old(Heap), Heap);
 
-// Item functions for different number of arguments
+procedure function.item_1<T1, R> (Current: ref, arg1: T1) returns (Result: R);
+  requires attached(Heap, Current, FUNCTION); // info:type property for argument Current
+  requires routine.precondition_1(Heap, Current, arg1);
+  modifies Heap;
+  ensures function.postcondition_1(Heap, old(Heap), Current, arg1, Result);
+  free ensures global(Heap);
+  requires Frame#Subset(routine.modify_1(Heap, Current, arg1), writable); // type:pre tag:frame_writable
+  free ensures same_outside(old(Heap), Heap, routine.modify_1(old(Heap), Current, arg1));
+  free ensures HeapSucc(old(Heap), Heap);
 
-procedure function.item_0<resultType> (
-        Current: ref where Current != Void && Heap[Current,$allocated]     // The agent object
-    ) returns (Result: resultType);
-    requires routine.precondition_0(Heap, Current);
-    modifies Heap;
-    ensures frame.modifies_agent(Heap, old(Heap), Current); // frame FUNCTION:item
-    ensures function.postcondition_0(Heap, old(Heap), Current, Result);
+procedure function.item_2<T1, T2, R> (Current: ref, arg1: T1, arg2: T2) returns (Result: R);
+  requires attached(Heap, Current, FUNCTION); // info:type property for argument Current
+  requires routine.precondition_2(Heap, Current, arg1, arg2);
+  modifies Heap;
+  ensures function.postcondition_2(Heap, old(Heap), Current, arg1, arg2, Result);
+  free ensures global(Heap);
+  requires Frame#Subset(routine.modify_2(Heap, Current, arg1, arg2), writable); // type:pre tag:frame_writable
+  free ensures same_outside(old(Heap), Heap, routine.modify_2(old(Heap), Current, arg1, arg2));
+  free ensures HeapSucc(old(Heap), Heap);
 
-procedure function.item_1<arg1Type, resultType> (
-        Current: ref where Current != Void && Heap[Current,$allocated],     // The agent object
-        arg1: arg1Type                                                           // First argument
-    ) returns (Result: resultType);
-    requires routine.precondition_1(Heap, Current, arg1);
-    modifies Heap;
-    ensures frame.modifies_agent(Heap, old(Heap), Current); // frame FUNCTION:item
-    ensures function.postcondition_1(Heap, old(Heap), Current, arg1, Result);
-
-procedure function.item_2<arg1Type, arg2Type, resultType> (
-        Current: ref where Current != Void && Heap[Current,$allocated],     // The agent object
-        arg1: arg1Type,                                                          // First argument
-        arg2: arg2Type                                                           // Second argument
-    ) returns (Result: resultType);
-    requires routine.precondition_2(Heap, Current, arg1, arg2);
-    modifies Heap;
-    ensures frame.modifies_agent(Heap, old(Heap), Current); // frame FUNCTION:item
-    ensures function.postcondition_2(Heap, old(Heap), Current, arg1, arg2, Result);
-
-procedure function.item_3<arg1Type, arg2Type, arg3Type, resultType> (
-        Current: ref where Current != Void && Heap[Current,$allocated],     // The agent object
-        arg1: arg1Type,                                                          // First argument
-        arg2: arg2Type,                                                          // Second argument
-        arg3: arg3Type                                                           // Third argument
-    ) returns (Result: resultType);
-    requires routine.precondition_3(Heap, Current, arg1, arg2, arg3);
-    modifies Heap;
-    ensures frame.modifies_agent(Heap, old(Heap), Current); // frame FUNCTION:item
-    ensures function.postcondition_3(Heap, old(Heap), Current, arg1, arg2, arg3, Result);
-
-	
-// ----------------------------------------------------------------------
-// Frame conditions
-
-// Frame condition for a feature which modifies only the `Current' object.
-function frame.modifies_current(heap: HeapType, old_heap: HeapType, current: ref) returns (bool);
-axiom (forall heap: HeapType, old_heap: HeapType, current: ref :: 
-            { frame.modifies_current(heap, old_heap, current) } // Trigger
-        frame.modifies_current(heap, old_heap, current) <==> 
-            (forall<alpha> $o: ref, $f: Field alpha :: 
-                    { heap[$o, $f] } // Trigger
-                ($o != Void && IsAllocated(old_heap, $o) && $o != current) ==> (old_heap[$o, $f] == heap[$o, $f])));
-
-// Frame condition for a feature which modifies what the `agent' modifies.
-function frame.modifies_agent(heap: HeapType, old_heap: HeapType, agent: ref) returns (bool);
-axiom (forall heap: HeapType, old_heap: HeapType, agent: ref :: 
-            { frame.modifies_agent(heap, old_heap, agent) } // Trigger
-        frame.modifies_agent(heap, old_heap, agent) <==> 
-            (forall<alpha> $o: ref, $f: Field alpha :: 
-                    { heap[$o, $f] } // Trigger
-                ($o != Void && IsAllocated(old_heap, $o) && !agent.modifies_0(heap, old_heap, agent, $o, $f)) ==> (old_heap[$o, $f] == heap[$o, $f])));
 
