eve/Src/framework/eiffel2boogie/tests/examples/vstte2008/vstte2008.e
@@ -97,4 +97,109 @@ feature -- VSTTE 2008: Adding and Multiplying Numbers
 			result_correct: Result = a * b
 		end
 
+feature -- VSTTE2008: Binary search
+
+	client_binary_search
+			-- Using binary search.
+		note
+			explicit: wrapping
+		local
+			a: SIMPLE_ARRAY [INTEGER]
+			i: INTEGER
+		do
+			create a.init (<<-3, 5, 9, 22, 104, 105, 107, 213>>)
+
+			i := binary_search (a, -3)
+			check i = 1 end
+			i := binary_search (a, 22)
+			check i = 4 end
+			i := binary_search (a, 56)
+			check i = 0 end
+		end
+
+	binary_search (a: SIMPLE_ARRAY [INTEGER]; x: INTEGER): INTEGER
+			-- Calculate index of `x' in `a', or return 0 if not found.
+		note
+			status: impure
+		require
+			a_not_void: a /= Void
+			a_sorted: sorted (a)
+		local
+			low, up, middle: INTEGER
+		do
+			from
+				low := 1
+				up := a.count + 1
+			invariant
+				low_and_up_range: 1 <= low and low <= up and up <= a.sequence.count + 1
+				result_range: Result = 0 or 1 <= Result and Result <= a.sequence.count
+				x_not_in_lower_part: across 1 |..| (low-1) as i all a.sequence[i.item] < x end
+				x_not_in_upper_part: across up |..| a.sequence.count as i all x < a.sequence[i.item] end
+				x_found: Result > 0 implies a.sequence[Result] = x
+			until
+				low >= up or Result > 0
+			loop
+				middle := low + ((up - low) // 2)
+				if a[middle] < x then
+					lemma_smaller_until_index (a, middle, x)
+					low := middle + 1
+				elseif a[middle] > x then
+					lemma_larger_from_index (a, middle, x)
+					up := middle
+				else
+					Result := middle
+				end
+			variant
+				(a.count - Result) + (up - low)
+			end
+		ensure
+			Result = 0 or 1 <= Result and Result <= a.sequence.count
+			Result = 0 implies not a.sequence.has (x)
+			Result > 0 implies a.sequence[Result] = x
+		end
+
+	sorted (a: SIMPLE_ARRAY [INTEGER]): BOOLEAN
+			-- Is `a' sorted?
+		note
+			status: functional
+		require
+			a /= Void
+		do
+			Result := across 1 |..| (a.sequence.count-1) as i all a.sequence[i.item] <= a.sequence[i.item+1] end
+		end
+
+	lemma_smaller_until_index (a: SIMPLE_ARRAY [INTEGER]; i, x: INTEGER)
+		note
+			status: lemma
+		require
+			a_wrapped: a.is_wrapped
+			a_sorted: sorted (a)
+			i_in_range: 1 <= i and i <= a.count
+			a_at_i_smaller: a.sequence[i] < x
+		do
+			if i > 1 then
+				lemma_smaller_until_index (a, i-1, x)
+			end
+		ensure
+			 a_until_i_smaller: across 1 |..| i as ai all a.sequence[ai.item] < x end
+		end
+
+	lemma_larger_from_index (a: SIMPLE_ARRAY [INTEGER]; i, x: INTEGER)
+		note
+			status: lemma
+		require
+			a_wrapped: a.is_wrapped
+			a_sorted: sorted (a)
+			i_in_range: 1 <= i and i <= a.count
+			a_at_i_larger: a.sequence[i] > x
+
+			decreases (a.count - i)
+		do
+			if i < a.sequence.count then
+				lemma_larger_from_index (a, i+1, x)
+			end
+		ensure
+			 a_from_i_larger: across i |..| a.sequence.count as ai all a.sequence[ai.item] > x end
+		end
+
 end
